model/fstar/README.md
@@ -1,0 +1,22 @@
+Proofs with MLS*
+================
+
+Verifying the proofs
+--------------------
+
+These proofs build on top of MLS\*, available here: https://github.com/Inria-Prosecco/treesync .
+Copy the files in `mls-star/fstar/treesync/code`,
+and follow the instructions to build it.
+
+Membership proof
+----------------
+
+The theorem `membership_proof_to_tree_hash_security` states that:
+given a root tree hash and a membership proof that verifies with it (`check_membership_proof`),
+for all trees with the same root tree hash,
+either the tree height is the same as the membership proof length
+and the tree contains the leaf node and parent nodes stored inside the membership proof (`membership_proof_guarantees`),
+or we can compute a hash collision (in polynomial time).
+
+The theorem also works for subtrees,
+in that case it also guarantees the position of the subtree.
